theory issue55 extends \root

context
  let one: 'one = ğ’« âˆ…'
  val x =  
      '(((((âˆ€ x. Â¬ (x âˆˆ âˆ…)) âˆ§ (one = (ğ’« âˆ…))) âˆ§ (âˆ€ x. âˆ€ y. ((x âˆˆ (ğ’« y)) âˆ¨ (Â¬ (x âŠ‚ y))) âˆ§ ((Â¬ (x âˆˆ (ğ’« y))) âˆ¨ (x âŠ‚ y)))) âˆ§ (âˆ€ x. âˆ€ y. ((x âŠ‚ y) âˆ¨ (Â¬ (âˆ€ z âˆˆ x. z âˆˆ y))) âˆ§ ((Â¬ (x âŠ‚ y)) âˆ¨ (âˆ€ z âˆˆ x. z âˆˆ y)))) âˆ§ (âˆ€ x_4. âˆ€ y_1. ((x_4 = y_1) âˆ¨ (âˆƒ x_2. Â¬ ((x_1 â†¦ (x_1 âˆˆ x_4) = (x_1 âˆˆ y_1)) x_2))) âˆ§ ((Â¬ (x_4 = y_1)) âˆ¨ (âˆ€ z. ((z âˆˆ x_4) âˆ¨ (Â¬ (z âˆˆ y_1))) âˆ§ ((Â¬ (z âˆˆ x_4)) âˆ¨ (z âˆˆ y_1)))))) âˆ§ (âˆƒ x_2. Â¬ ((x_1 â†¦ (x_1 âˆˆ one) = (x_1 = âˆ…)) x_2))'      
  val y =  
      'âˆ€ x_6. âˆ€ x_5. âˆƒ x_3. âˆƒ y. âˆ€ x. ((x_2 â†¦ (((Â¬ ((x_3 âˆˆ x_6) = (x_3 âˆˆ x_5))) âˆ¨ (x_6 = x_5)) âˆ§ ((((x_2 âˆˆ x_6) âˆ¨ (Â¬ (x_2 âˆˆ x_5))) âˆ§ ((Â¬ (x_2 âˆˆ x_6)) âˆ¨ (x_2 âˆˆ x_5))) âˆ¨ (Â¬ (x_6 = x_5)))) âˆ§ (((((x_6 âˆˆ (ğ’« x_5)) âˆ¨ (Â¬ (x_6 âŠ‚ x_5))) âˆ§ ((Â¬ (x_6 âˆˆ (ğ’« x_5))) âˆ¨ (x_6 âŠ‚ x_5))) âˆ§ ((Â¬ (x_6 âˆˆ âˆ…)) âˆ§ (one = (ğ’« âˆ…)))) âˆ§ (((x_6 âŠ‚ x_5) âˆ¨ (Â¬ (âˆ€ z âˆˆ x_6. z âˆˆ x_5))) âˆ§ ((Â¬ (x_6 âŠ‚ x_5)) âˆ¨ (âˆ€ z âˆˆ x_6. z âˆˆ x_5))))) x) âˆ§ ((x â†¦ Â¬ ((y âˆˆ one) = (y = âˆ…))) x)'
  val t = 
      '((((((âˆ€ x. Â¬ (x âˆˆ âˆ…)) âˆ§ (one = (ğ’« âˆ…))) âˆ§ (âˆ€ x. âˆ€ y. ((x âˆˆ (ğ’« y)) âˆ¨ (Â¬ (x âŠ‚ y))) âˆ§ ((Â¬ (x âˆˆ (ğ’« y))) âˆ¨ (x âŠ‚ y)))) âˆ§ (âˆ€ x. âˆ€ y. ((x âŠ‚ y) âˆ¨ (Â¬ (âˆ€ z âˆˆ x. z âˆˆ y))) âˆ§ ((Â¬ (x âŠ‚ y)) âˆ¨ (âˆ€ z âˆˆ x. z âˆˆ y)))) âˆ§ (âˆ€ x_4. âˆ€ y_1. ((x_4 = y_1) âˆ¨ (âˆƒ x_2. Â¬ ((x_1 â†¦ (x_1 âˆˆ x_4) = (x_1 âˆˆ y_1)) x_2))) âˆ§ ((Â¬ (x_4 = y_1)) âˆ¨ (âˆ€ z. ((z âˆˆ x_4) âˆ¨ (Â¬ (z âˆˆ y_1))) âˆ§ ((Â¬ (z âˆˆ x_4)) âˆ¨ (z âˆˆ y_1)))))) âˆ§ (âˆƒ x_2. Â¬ ((x_1 â†¦ (x_1 âˆˆ one) = (x_1 = âˆ…)) x_2))) = (âˆ€ x_6. âˆ€ x_5. âˆƒ x_3. âˆƒ y. âˆ€ x. ((x_2 â†¦ (((Â¬ ((x_3 âˆˆ x_6) = (x_3 âˆˆ x_5))) âˆ¨ (x_6 = x_5)) âˆ§ ((((x_2 âˆˆ x_6) âˆ¨ (Â¬ (x_2 âˆˆ x_5))) âˆ§ ((Â¬ (x_2 âˆˆ x_6)) âˆ¨ (x_2 âˆˆ x_5))) âˆ¨ (Â¬ (x_6 = x_5)))) âˆ§ (((((x_6 âˆˆ (ğ’« x_5)) âˆ¨ (Â¬ (x_6 âŠ‚ x_5))) âˆ§ ((Â¬ (x_6 âˆˆ (ğ’« x_5))) âˆ¨ (x_6 âŠ‚ x_5))) âˆ§ ((Â¬ (x_6 âˆˆ âˆ…)) âˆ§ (one = (ğ’« âˆ…)))) âˆ§ (((x_6 âŠ‚ x_5) âˆ¨ (Â¬ (âˆ€ z âˆˆ x_6. z âˆˆ x_5))) âˆ§ ((Â¬ (x_6 âŠ‚ x_5)) âˆ¨ (âˆ€ z âˆˆ x_6. z âˆˆ x_5))))) x) âˆ§ ((x â†¦ Â¬ ((y âˆˆ one) = (y = âˆ…))) x))'
  assume th: t
  timeit
    val s 
    timeit
      s = 'â€¹xâ€º = â€¹yâ€º'
    timeit
      theorem foo: s
        th
      foo

# The timings resulting for this code before dealing with this issue are:

  start compiling theory '\issues\issue55' ...
    ** timeit (\issues\issue55:14): 462ms
    ** timeit (\issues\issue55:16): 9ms
    ** timeit (\issues\issue55:12): 475ms
  successfully compiled theory '\issues\issue55'

